Monad.v
@@ -2,24 +2,24 @@ Require Import Utf8.
 Require Import AbstractStore.
 
 
-Definition State {S : Type} (A : Type) := S -> option (A * S)%type.
+Definition State (S : Type) (A : Type) := S -> option (A * S)%type.
 
-Definition return_state {S A : Type} (x : A) : State A :=
+Definition return_state (S A : Type) (x : A) : State S A :=
   fun (st : S) => Some (x, st).
 
-Definition bind_state {S A B : Type} (m : @State S A) (f : A -> @State S B) 
-    : State B :=
+Definition bind_state (S A B : Type) (m : State S A) (f : A -> State S B) 
+    : State S B :=
   fun st => match m st with
             | Some (x, st') => f x st'
             | None => None
             end.
 
-Definition get {S : Type} : State S := fun st => Some (st, st).
+Definition get {S : Type} : State S S := fun st => Some (st, st).
 
-Definition put {S : Type} (st' : S) : @State S unit := 
+Definition put {S : Type} (st' : S) : State S unit := 
   fun st => Some (tt, st').
 
-Definition fail {S A : Type} : @State S A :=
+Definition fail {S A : Type} : State S A :=
   fun st => None.
 
  
@@ -32,9 +32,9 @@ Arguments Build_Monad {_ _ _}.
 Arguments returnM {_ _ _}.
 Arguments bind {_ _ _ _}.
 
-Instance state_monad {S : Type} : Monad (@State S) := {
-  returnM := (@return_state S);
-  bind := (@bind_state S);
+Instance state_monad {S : Type} : Monad (State S) := {
+  returnM := (return_state S);
+  bind := (bind_state S);
 }.
 
 Notation "x '<<' y ; z" := (bind y (fun x => z))
